Flags example cleanup.

theories/examples/misc/flags.c
@@ -1,43 +1,36 @@
 #include <stdint.h>
 
 //@rc::inlined
-//@Definition flags_type := (bool * bool * bool)%type.
+//@Record Flags := mkFlags {
+//@  flag1 : bool ;
+//@  flag2 : bool ;
+//@}.
 //@
-//@Definition flags_from_nat n :=
-//@  let b0 := bool_decide (n `mod` 2 = 1) in
-//@  let n  := n `div` 2 in
-//@  let b1 := bool_decide (n `mod` 2 = 1) in
-//@  let n  := n `div` 2 in
-//@  let b2 := bool_decide (n `mod` 2 = 1) in
-//@  let n  := n `div` 2 in
-//@  if bool_decide (n = 0) then Some (b0, b1, b2) else None.
+//@Definition nat_encodes_flags n fs :=
+//@  Z.testbit 0 n = flag1 fs ∧
+//@  Z.testbit 1 n = flag2 fs ∧
+//@  ∀ k, k > 1 → ¬ Z.testbit k n.
 //@rc::end
 
 typedef struct
-[[rc::refined_by("f : flags_type")]]
+[[rc::refined_by("f : Flags")]]
 [[rc::exists("n : nat")]]
-[[rc::constraints("{flags_from_nat n = Some f}")]]
+[[rc::constraints("{nat_encodes_flags n f}")]]
 flags {
   [[rc::field("n @ int<u8>")]]
   uint8_t flags;
 } flags_t;
 
-#define IS_SET(f, n) (((f).flags >> (n)) % 2 == 1)
+#define IS_SET(f, n) (((f).flags >> (n)) & 1)
 
-[[rc::parameters("f1 : bool", "f2 : bool", "f3 : bool")]]
-[[rc::parameters("n1 : nat", "n2 : nat", "n3 : nat")]]
-[[rc::args("{(f1, f2, f3)} @ flags")]]
-[[rc::args("n1 @ int<u32>", "n2 @ int<u32>", "n3 @ int<u32>")]]
+[[rc::parameters("fs : Flags", "n1 : nat", "n2 : nat")]]
+[[rc::args("fs @ flags", "n1 @ int<u32>", "n2 @ int<u32>")]]
 [[rc::requires("{n1 + n2 < it_max u32}")]]
-[[rc::requires("{n2 + n3 < it_max u32}")]]
-[[rc::requires("{n1 + n3 < it_max u32}")]]
-[[rc::requires("{n1 + n2 + n3 < it_max u32}")]]
-[[rc::returns("{(if f1 then n1 else 0) + (if f2 then n2 else 0) + (if f3 then n3 else 0)} @ int<u32>")]]
+[[rc::returns("{(if flag1 fs then n1 else 0) + (if flag2 fs then n2 else 0)} @ int<u32>")]]
 [[rc::trust_me]] // FIXME automation
-unsigned int sum(flags_t f, unsigned int arg1, unsigned int arg2, unsigned int arg3){
+unsigned int sum(flags_t f, unsigned int arg1, unsigned int arg2){
   unsigned int r = 0;
   if(IS_SET(f, 0)) r += arg1;
   if(IS_SET(f, 1)) r += arg2;
-  if(IS_SET(f, 2)) r += arg3;
   return r;
 }
