theories/examples/misc/flags_spec.v
@@ -8,24 +8,23 @@ Section spec.
 
   (* Inlined code. *)
 
-  Definition flags_type := (bool * bool * bool)%type.
+  Record Flags := mkFlags {
+    flag1 : bool ;
+    flag2 : bool ;
+  }.
 
-  Definition flags_from_nat n :=
-    let b0 := bool_decide (n `mod` 2 = 1) in
-    let n  := n `div` 2 in
-    let b1 := bool_decide (n `mod` 2 = 1) in
-    let n  := n `div` 2 in
-    let b2 := bool_decide (n `mod` 2 = 1) in
-    let n  := n `div` 2 in
-    if bool_decide (n = 0) then Some (b0, b1, b2) else None.
+  Definition nat_encodes_flags n fs :=
+    Z.testbit 0 n = flag1 fs ∧
+    Z.testbit 1 n = flag2 fs ∧
+    ∀ k, k > 1 → ¬ Z.testbit k n.
 
   (* Definition of type [flags]. *)
-  Definition flags_rec : (flags_type -d> typeO) → (flags_type -d> typeO) := (λ self f,
+  Definition flags_rec : (Flags -d> typeO) → (Flags -d> typeO) := (λ self f,
     tyexists (λ n : nat,
     constrained (struct struct_flags [@{type}
       (n @ (int (u8)))
     ]) (
-      ⌜flags_from_nat n = Some f⌝
+      ⌜nat_encodes_flags n f⌝
     ))
   )%I.
   Typeclasses Opaque flags_rec.
@@ -34,17 +33,17 @@ Section spec.
   Proof. solve_type_proper. Qed.
 
   Definition flags : rtype := {|
-    rty_type := flags_type;
+    rty_type := Flags;
     rty r__ := fixp flags_rec r__
   |}.
 
-  Lemma flags_unfold (f : flags_type) :
+  Lemma flags_unfold (f : Flags) :
     (f @ flags)%I ≡@{type} (
       tyexists (λ n : nat,
       constrained (struct struct_flags [@{type}
         (n @ (int (u8)))
       ]) (
-        ⌜flags_from_nat n = Some f⌝
+        ⌜nat_encodes_flags n f⌝
       ))
     )%I.
   Proof. by rewrite {1}/with_refinement/=fixp_unfold. Qed.
@@ -54,18 +53,18 @@ Section spec.
     {| rmovable 'f := movable_eq _ _ (flags_unfold f) |}.
   Next Obligation. solve_ty_layout_eq. Qed.
 
-  Global Instance flags_simplify_hyp_place_inst l_ β_ (f : flags_type) :
+  Global Instance flags_simplify_hyp_place_inst l_ β_ (f : Flags) :
     SimplifyHypPlace l_ β_ (f @ flags)%I (Some 100%N) :=
     λ T, i2p (simplify_hyp_place_eq l_ β_ _ _ T (flags_unfold _)).
-  Global Instance flags_simplify_goal_place_inst l_ β_ (f : flags_type) :
+  Global Instance flags_simplify_goal_place_inst l_ β_ (f : Flags) :
     SimplifyGoalPlace l_ β_ (f @ flags)%I (Some 100%N) :=
     λ T, i2p (simplify_goal_place_eq l_ β_ _ _ T (flags_unfold _)).
 
-  Global Program Instance flags_simplify_hyp_val_inst v_ (f : flags_type) :
+  Global Program Instance flags_simplify_hyp_val_inst v_ (f : Flags) :
     SimplifyHypVal v_ (f @ flags)%I (Some 100%N) :=
     λ T, i2p (simplify_hyp_val_eq v_ _ _ (flags_unfold _) T _).
   Next Obligation. done. Qed.
-  Global Program Instance flags_simplify_goal_val_inst v_ (f : flags_type) :
+  Global Program Instance flags_simplify_goal_val_inst v_ (f : Flags) :
     SimplifyGoalVal v_ (f @ flags)%I (Some 100%N) :=
     λ T, i2p (simplify_goal_val_eq v_ _ _ (flags_unfold _) T _).
   Next Obligation. done. Qed.
@@ -74,8 +73,8 @@ Section spec.
 
   (* Specifications for function [sum]. *)
   Definition type_of_sum :=
-    fn(∀ (f1, f2, f3, n1, n2, n3) : bool * bool * bool * nat * nat * nat; (((f1, f2, f3)) @ (flags)), (n1 @ (int (u32))), (n2 @ (int (u32))), (n3 @ (int (u32))); ⌜n1 + n2 < it_max u32⌝ ∗ ⌜n2 + n3 < it_max u32⌝ ∗ ⌜n1 + n3 < it_max u32⌝ ∗ ⌜n1 + n2 + n3 < it_max u32⌝)
-      → ∃ () : (), (((if f1 then n1 else 0) + (if f2 then n2 else 0) + (if f3 then n3 else 0)) @ (int (u32))); True.
+    fn(∀ (fs, n1, n2) : Flags * nat * nat; (fs @ (flags)), (n1 @ (int (u32))), (n2 @ (int (u32))); ⌜n1 + n2 < it_max u32⌝)
+      → ∃ () : (), (((if flag1 fs then n1 else 0) + (if flag2 fs then n2 else 0)) @ (int (u32))); True.
 End spec.
 
 Typeclasses Opaque flags_rec.
