theories/examples/misc/flags_code.v
@@ -6,62 +6,41 @@ Set Default Proof Using "Type".
 (* Generated from [theories/examples/misc/flags.c]. *)
 Section code.
   Definition file_0 : string := "theories/examples/misc/flags.c".
-  Definition loc_2 : location_info := LocationInfo file_0 38 2 38 21.
-  Definition loc_3 : location_info := LocationInfo file_0 39 2 39 46.
-  Definition loc_4 : location_info := LocationInfo file_0 40 2 40 46.
-  Definition loc_5 : location_info := LocationInfo file_0 41 2 41 46.
-  Definition loc_6 : location_info := LocationInfo file_0 42 2 42 11.
-  Definition loc_7 : location_info := LocationInfo file_0 42 9 42 10.
-  Definition loc_8 : location_info := LocationInfo file_0 42 9 42 10.
-  Definition loc_9 : location_info := LocationInfo file_0 41 36 41 46.
-  Definition loc_10 : location_info := LocationInfo file_0 41 36 41 37.
-  Definition loc_11 : location_info := LocationInfo file_0 41 36 41 45.
-  Definition loc_12 : location_info := LocationInfo file_0 41 36 41 37.
-  Definition loc_13 : location_info := LocationInfo file_0 41 36 41 37.
-  Definition loc_14 : location_info := LocationInfo file_0 41 41 41 45.
-  Definition loc_15 : location_info := LocationInfo file_0 41 41 41 45.
-  Definition loc_17 : location_info := LocationInfo file_0 41 5 41 34.
-  Definition loc_18 : location_info := LocationInfo file_0 41 6 41 28.
-  Definition loc_19 : location_info := LocationInfo file_0 41 6 41 24.
-  Definition loc_20 : location_info := LocationInfo file_0 41 7 41 16.
-  Definition loc_21 : location_info := LocationInfo file_0 41 7 41 16.
-  Definition loc_22 : location_info := LocationInfo file_0 41 7 41 10.
-  Definition loc_23 : location_info := LocationInfo file_0 41 20 41 23.
-  Definition loc_24 : location_info := LocationInfo file_0 41 27 41 28.
-  Definition loc_25 : location_info := LocationInfo file_0 41 32 41 33.
-  Definition loc_26 : location_info := LocationInfo file_0 40 36 40 46.
-  Definition loc_27 : location_info := LocationInfo file_0 40 36 40 37.
-  Definition loc_28 : location_info := LocationInfo file_0 40 36 40 45.
-  Definition loc_29 : location_info := LocationInfo file_0 40 36 40 37.
-  Definition loc_30 : location_info := LocationInfo file_0 40 36 40 37.
-  Definition loc_31 : location_info := LocationInfo file_0 40 41 40 45.
-  Definition loc_32 : location_info := LocationInfo file_0 40 41 40 45.
-  Definition loc_34 : location_info := LocationInfo file_0 40 5 40 34.
-  Definition loc_35 : location_info := LocationInfo file_0 40 6 40 28.
-  Definition loc_36 : location_info := LocationInfo file_0 40 6 40 24.
-  Definition loc_37 : location_info := LocationInfo file_0 40 7 40 16.
-  Definition loc_38 : location_info := LocationInfo file_0 40 7 40 16.
-  Definition loc_39 : location_info := LocationInfo file_0 40 7 40 10.
-  Definition loc_40 : location_info := LocationInfo file_0 40 20 40 23.
-  Definition loc_41 : location_info := LocationInfo file_0 40 27 40 28.
-  Definition loc_42 : location_info := LocationInfo file_0 40 32 40 33.
-  Definition loc_43 : location_info := LocationInfo file_0 39 36 39 46.
-  Definition loc_44 : location_info := LocationInfo file_0 39 36 39 37.
-  Definition loc_45 : location_info := LocationInfo file_0 39 36 39 45.
-  Definition loc_46 : location_info := LocationInfo file_0 39 36 39 37.
-  Definition loc_47 : location_info := LocationInfo file_0 39 36 39 37.
-  Definition loc_48 : location_info := LocationInfo file_0 39 41 39 45.
-  Definition loc_49 : location_info := LocationInfo file_0 39 41 39 45.
-  Definition loc_51 : location_info := LocationInfo file_0 39 5 39 34.
-  Definition loc_52 : location_info := LocationInfo file_0 39 6 39 28.
-  Definition loc_53 : location_info := LocationInfo file_0 39 6 39 24.
-  Definition loc_54 : location_info := LocationInfo file_0 39 7 39 16.
-  Definition loc_55 : location_info := LocationInfo file_0 39 7 39 16.
-  Definition loc_56 : location_info := LocationInfo file_0 39 7 39 10.
-  Definition loc_57 : location_info := LocationInfo file_0 39 20 39 23.
-  Definition loc_58 : location_info := LocationInfo file_0 39 27 39 28.
-  Definition loc_59 : location_info := LocationInfo file_0 39 32 39 33.
-  Definition loc_60 : location_info := LocationInfo file_0 38 19 38 20.
+  Definition loc_2 : location_info := LocationInfo file_0 32 2 32 21.
+  Definition loc_3 : location_info := LocationInfo file_0 33 2 33 41.
+  Definition loc_4 : location_info := LocationInfo file_0 34 2 34 41.
+  Definition loc_5 : location_info := LocationInfo file_0 35 2 35 11.
+  Definition loc_6 : location_info := LocationInfo file_0 35 9 35 10.
+  Definition loc_7 : location_info := LocationInfo file_0 35 9 35 10.
+  Definition loc_8 : location_info := LocationInfo file_0 34 31 34 41.
+  Definition loc_9 : location_info := LocationInfo file_0 34 31 34 32.
+  Definition loc_10 : location_info := LocationInfo file_0 34 31 34 40.
+  Definition loc_11 : location_info := LocationInfo file_0 34 31 34 32.
+  Definition loc_12 : location_info := LocationInfo file_0 34 31 34 32.
+  Definition loc_13 : location_info := LocationInfo file_0 34 36 34 40.
+  Definition loc_14 : location_info := LocationInfo file_0 34 36 34 40.
+  Definition loc_16 : location_info := LocationInfo file_0 34 5 34 29.
+  Definition loc_17 : location_info := LocationInfo file_0 34 6 34 24.
+  Definition loc_18 : location_info := LocationInfo file_0 34 7 34 16.
+  Definition loc_19 : location_info := LocationInfo file_0 34 7 34 16.
+  Definition loc_20 : location_info := LocationInfo file_0 34 7 34 10.
+  Definition loc_21 : location_info := LocationInfo file_0 34 20 34 23.
+  Definition loc_22 : location_info := LocationInfo file_0 34 27 34 28.
+  Definition loc_23 : location_info := LocationInfo file_0 33 31 33 41.
+  Definition loc_24 : location_info := LocationInfo file_0 33 31 33 32.
+  Definition loc_25 : location_info := LocationInfo file_0 33 31 33 40.
+  Definition loc_26 : location_info := LocationInfo file_0 33 31 33 32.
+  Definition loc_27 : location_info := LocationInfo file_0 33 31 33 32.
+  Definition loc_28 : location_info := LocationInfo file_0 33 36 33 40.
+  Definition loc_29 : location_info := LocationInfo file_0 33 36 33 40.
+  Definition loc_31 : location_info := LocationInfo file_0 33 5 33 29.
+  Definition loc_32 : location_info := LocationInfo file_0 33 6 33 24.
+  Definition loc_33 : location_info := LocationInfo file_0 33 7 33 16.
+  Definition loc_34 : location_info := LocationInfo file_0 33 7 33 16.
+  Definition loc_35 : location_info := LocationInfo file_0 33 7 33 10.
+  Definition loc_36 : location_info := LocationInfo file_0 33 20 33 23.
+  Definition loc_37 : location_info := LocationInfo file_0 33 27 33 28.
+  Definition loc_38 : location_info := LocationInfo file_0 32 19 32 20.
 
   (* Definition of struct [flags]. *)
   Program Definition struct_flags := {|
@@ -76,8 +55,7 @@ Section code.
     f_args := [
       ("f", layout_of struct_flags);
       ("arg1", it_layout u32);
-      ("arg2", it_layout u32);
-      ("arg3", it_layout u32)
+      ("arg2", it_layout u32)
     ];
     f_local_vars := [
       ("r", it_layout u32)
@@ -86,71 +64,50 @@ Section code.
     f_code := (
       <[ "#0" :=
         "r" <-{ it_layout u32 }
-          LocInfoE loc_60 (UnOp (CastOp $ IntOp u32) (IntOp i32) (LocInfoE loc_60 (i2v 0 i32))) ;
-        locinfo: loc_51 ;
-        if: LocInfoE loc_51 (UnOp (CastOp $ IntOp bool_it) (IntOp i32) (LocInfoE loc_51 ((LocInfoE loc_52 ((LocInfoE loc_53 ((LocInfoE loc_54 (UnOp (CastOp $ IntOp i32) (IntOp u8) (LocInfoE loc_54 (use{it_layout u8} (LocInfoE loc_55 ((LocInfoE loc_56 ("f")) at{struct_flags} "flags")))))) >>{IntOp i32, IntOp i32} (LocInfoE loc_57 (i2v 0 i32)))) %{IntOp i32, IntOp i32} (LocInfoE loc_58 (i2v 2 i32)))) ={IntOp i32, IntOp i32} (LocInfoE loc_59 (i2v 1 i32)))))
+          LocInfoE loc_38 (UnOp (CastOp $ IntOp u32) (IntOp i32) (LocInfoE loc_38 (i2v 0 i32))) ;
+        locinfo: loc_31 ;
+        if: LocInfoE loc_31 (UnOp (CastOp $ IntOp bool_it) (IntOp i32) (LocInfoE loc_31 ((LocInfoE loc_32 ((LocInfoE loc_33 (UnOp (CastOp $ IntOp i32) (IntOp u8) (LocInfoE loc_33 (use{it_layout u8} (LocInfoE loc_34 ((LocInfoE loc_35 ("f")) at{struct_flags} "flags")))))) >>{IntOp i32, IntOp i32} (LocInfoE loc_36 (i2v 0 i32)))) &{IntOp i32, IntOp i32} (LocInfoE loc_37 (i2v 1 i32)))))
         then
-        locinfo: loc_43 ;
-          Goto "#8"
+        locinfo: loc_23 ;
+          Goto "#5"
         else
-        locinfo: loc_34 ;
-          Goto "#9"
+        locinfo: loc_16 ;
+          Goto "#6"
       ]> $
       <[ "#1" :=
-        locinfo: loc_34 ;
-        if: LocInfoE loc_34 (UnOp (CastOp $ IntOp bool_it) (IntOp i32) (LocInfoE loc_34 ((LocInfoE loc_35 ((LocInfoE loc_36 ((LocInfoE loc_37 (UnOp (CastOp $ IntOp i32) (IntOp u8) (LocInfoE loc_37 (use{it_layout u8} (LocInfoE loc_38 ((LocInfoE loc_39 ("f")) at{struct_flags} "flags")))))) >>{IntOp i32, IntOp i32} (LocInfoE loc_40 (i2v 1 i32)))) %{IntOp i32, IntOp i32} (LocInfoE loc_41 (i2v 2 i32)))) ={IntOp i32, IntOp i32} (LocInfoE loc_42 (i2v 1 i32)))))
+        locinfo: loc_16 ;
+        if: LocInfoE loc_16 (UnOp (CastOp $ IntOp bool_it) (IntOp i32) (LocInfoE loc_16 ((LocInfoE loc_17 ((LocInfoE loc_18 (UnOp (CastOp $ IntOp i32) (IntOp u8) (LocInfoE loc_18 (use{it_layout u8} (LocInfoE loc_19 ((LocInfoE loc_20 ("f")) at{struct_flags} "flags")))))) >>{IntOp i32, IntOp i32} (LocInfoE loc_21 (i2v 1 i32)))) &{IntOp i32, IntOp i32} (LocInfoE loc_22 (i2v 1 i32)))))
         then
-        locinfo: loc_26 ;
-          Goto "#6"
+        locinfo: loc_8 ;
+          Goto "#3"
         else
-        locinfo: loc_17 ;
-          Goto "#7"
+        locinfo: loc_5 ;
+          Goto "#4"
       ]> $
       <[ "#2" :=
-        locinfo: loc_17 ;
-        if: LocInfoE loc_17 (UnOp (CastOp $ IntOp bool_it) (IntOp i32) (LocInfoE loc_17 ((LocInfoE loc_18 ((LocInfoE loc_19 ((LocInfoE loc_20 (UnOp (CastOp $ IntOp i32) (IntOp u8) (LocInfoE loc_20 (use{it_layout u8} (LocInfoE loc_21 ((LocInfoE loc_22 ("f")) at{struct_flags} "flags")))))) >>{IntOp i32, IntOp i32} (LocInfoE loc_23 (i2v 2 i32)))) %{IntOp i32, IntOp i32} (LocInfoE loc_24 (i2v 2 i32)))) ={IntOp i32, IntOp i32} (LocInfoE loc_25 (i2v 1 i32)))))
-        then
-        locinfo: loc_9 ;
-          Goto "#4"
-        else
-        locinfo: loc_6 ;
-          Goto "#5"
+        locinfo: loc_5 ;
+        Return (LocInfoE loc_6 (use{it_layout u32} (LocInfoE loc_7 ("r"))))
       ]> $
       <[ "#3" :=
-        locinfo: loc_6 ;
-        Return (LocInfoE loc_7 (use{it_layout u32} (LocInfoE loc_8 ("r"))))
+        locinfo: loc_8 ;
+        LocInfoE loc_9 ("r") <-{ it_layout u32 }
+          LocInfoE loc_10 ((LocInfoE loc_11 (use{it_layout u32} (LocInfoE loc_12 ("r")))) +{IntOp u32, IntOp u32} (LocInfoE loc_13 (use{it_layout u32} (LocInfoE loc_14 ("arg2"))))) ;
+        locinfo: loc_5 ;
+        Goto "#2"
       ]> $
       <[ "#4" :=
-        locinfo: loc_9 ;
-        LocInfoE loc_10 ("r") <-{ it_layout u32 }
-          LocInfoE loc_11 ((LocInfoE loc_12 (use{it_layout u32} (LocInfoE loc_13 ("r")))) +{IntOp u32, IntOp u32} (LocInfoE loc_14 (use{it_layout u32} (LocInfoE loc_15 ("arg3"))))) ;
-        locinfo: loc_6 ;
-        Goto "#3"
+        locinfo: loc_5 ;
+        Goto "#2"
       ]> $
       <[ "#5" :=
-        locinfo: loc_6 ;
-        Goto "#3"
-      ]> $
-      <[ "#6" :=
-        locinfo: loc_26 ;
-        LocInfoE loc_27 ("r") <-{ it_layout u32 }
-          LocInfoE loc_28 ((LocInfoE loc_29 (use{it_layout u32} (LocInfoE loc_30 ("r")))) +{IntOp u32, IntOp u32} (LocInfoE loc_31 (use{it_layout u32} (LocInfoE loc_32 ("arg2"))))) ;
-        locinfo: loc_17 ;
-        Goto "#2"
-      ]> $
-      <[ "#7" :=
-        locinfo: loc_17 ;
-        Goto "#2"
-      ]> $
-      <[ "#8" :=
-        locinfo: loc_43 ;
-        LocInfoE loc_44 ("r") <-{ it_layout u32 }
-          LocInfoE loc_45 ((LocInfoE loc_46 (use{it_layout u32} (LocInfoE loc_47 ("r")))) +{IntOp u32, IntOp u32} (LocInfoE loc_48 (use{it_layout u32} (LocInfoE loc_49 ("arg1"))))) ;
-        locinfo: loc_34 ;
+        locinfo: loc_23 ;
+        LocInfoE loc_24 ("r") <-{ it_layout u32 }
+          LocInfoE loc_25 ((LocInfoE loc_26 (use{it_layout u32} (LocInfoE loc_27 ("r")))) +{IntOp u32, IntOp u32} (LocInfoE loc_28 (use{it_layout u32} (LocInfoE loc_29 ("arg1"))))) ;
+        locinfo: loc_16 ;
         Goto "#1"
       ]> $
-      <[ "#9" :=
-        locinfo: loc_34 ;
+      <[ "#6" :=
+        locinfo: loc_16 ;
         Goto "#1"
       ]> $∅
     )%E
